progress.lean
@@ -11,19 +11,173 @@ lemma exp.vcgen.return.inv {P: prop} {x: var} {Q: propctx}: (P ⊢ exp.return x 
     }
   end
 
-lemma stack.vcgen.top.inv {P: prop} {σ: env} {e: exp}: (P ⊩ (σ, e)) → ∃P₂ Q, (⊢ σ: P₂) ∧ (P & P₂ ⊢ e: Q) :=
-  assume top_verified: P ⊩ (σ, e),
+lemma stack.vcgen.top.inv {H: list call} {σ: env} {e: exp}: (H ⊩ (σ, e)) → ∃P Q, (⊢ σ: P) ∧ (H & P ⊢ e: Q) :=
+  assume top_verified: H ⊩ (σ, e),
   begin
     cases top_verified,
-    case stack.vcgen.top P₂ Q env_verified e_verified { from
-      have (⊢ σ: P₂) ∧ (P & P₂ ⊢ e: Q), from ⟨env_verified, e_verified⟩,
-      show ∃P₂ Q, (⊢ σ: P₂) ∧ (P & P₂ ⊢ e: Q), from exists.intro P₂ $ exists.intro Q this
+    case stack.vcgen.top P Q env_verified e_verified {
+      show ∃P Q, (⊢ σ: P) ∧ (H & P ⊢ e: Q), from exists.intro P (exists.intro Q ⟨env_verified, e_verified⟩)
     }
   end
 
-theorem progress(P: prop) (s: stack): ⟪P⟫ ∧ (P ⊩ s) → is_return s ∨ ∃c s', s ⟶ c, s'
+lemma val_of_free_in_nonempty_env {P: prop} {σ: env} {x y: var} {v: value}:
+                                  (⊢ σ : P) → (x ≠ y → ∃v', σ y = some v') →
+                                  ∃v', σ[x↦v] y = some v' :=
+  assume env_verified: ⊢ σ : P,
+  assume ih: x ≠ y → ∃v', σ y = some v',
+  if x_eq_y: x = y then (
+    have h: σ[x↦v].apply x = (if x = x then ↑v else σ.apply x), by unfold env.apply,
+    have (if x = x then ↑v else σ.apply x) = ↑v, by simp *,
+    have σ[x↦v].apply x = ↑v, from this ▸ h,
+    have σ[x↦v].apply y = some v, from x_eq_y ▸ this,
+    show ∃v', σ[x↦v] y = some v', from exists.intro v this
+  ) else (
+    have ∃v', σ y = some v', from ih x_eq_y,
+    let ⟨v', σ_has_y⟩ := this in
+    have h: σ[x↦v].apply y = (if x = y then ↑v else σ.apply y), by unfold env.apply,
+    have (if x = y then ↑v else σ.apply y) = σ.apply y, by simp *,
+    have σ[x↦v].apply y = σ.apply y, from this ▸ h,
+    have σ[x↦v].apply y = some v', from eq.trans this σ_has_y,
+    show ∃v', σ[x↦v] y = some v', from exists.intro v' this
+  )
+
+lemma val_of_free_in_env {P: prop} {σ: env} {x: var}: (⊢ σ : P) → x ∈ FV P → ∃v, σ x = some v :=
+  assume env_verified: ⊢ σ: P,
+  assume x_free_in_P: x ∈ FV P,
+  begin
+    induction env_verified,
+    case env.vcgen.empty {
+      cases x_free_in_P,
+      case free_in_prop.term x_free_in_true {
+        cases x_free_in_true
+      }
+    },
+    case env.vcgen.tru σ' x' Q σ'_verified ih { from
+      val_of_free_in_nonempty_env σ'_verified (
+        assume x'_is_not_x: x' ≠ x,
+        have free_in_prop x Q ∨ free_in_prop x (x' ≡ value.true), from free_in_prop.and.inv x_free_in_P,
+        or.elim this.symm
+        (
+          assume x_free_in_true: free_in_prop x (x' ≡ value.true),
+          show ∃v, σ' x = some v, by begin
+            cases x_free_in_true,
+            case free_in_prop.term x_free_in_eq {
+              cases x_free_in_eq,
+              case free_in_term.binop₁ free_in_x' {
+                have x'_is_x: (x' = x), from (free_in_term.freevar.inv free_in_x').symm,
+                contradiction
+              },
+              case free_in_term.binop₂ free_in_true {
+                cases free_in_true
+              }
+            }
+          end
+        )
+        (
+          assume x_free_in_Q: free_in_prop x Q,
+          show ∃v, σ' x = some v, from ih x_free_in_Q
+        )
+      )
+    },
+    case env.vcgen.fls σ' x' Q σ'_verified ih { from
+      val_of_free_in_nonempty_env σ'_verified (
+        assume x'_is_not_x: x' ≠ x,
+        have free_in_prop x Q ∨ free_in_prop x (x' ≡ value.false), from free_in_prop.and.inv x_free_in_P,
+        or.elim this.symm
+        (
+          assume x_free_in_false: free_in_prop x (x' ≡ value.false),
+          show ∃v, σ' x = some v, by begin
+            cases x_free_in_false,
+            case free_in_prop.term x_free_in_eq {
+              cases x_free_in_eq,
+              case free_in_term.binop₁ free_in_x' {
+                have x'_is_x: (x' = x), from (free_in_term.freevar.inv free_in_x').symm,
+                contradiction
+              },
+              case free_in_term.binop₂ free_in_false {
+                cases free_in_false
+              }
+            }
+          end
+        )
+        (
+          assume x_free_in_Q: free_in_prop x Q,
+          show ∃v, σ' x = some v, from ih x_free_in_Q
+        )
+      )
+    },
+    case env.vcgen.num n σ' x' Q σ'_verified ih { from
+      val_of_free_in_nonempty_env σ'_verified (
+        assume x'_is_not_x: x' ≠ x,
+        have free_in_prop x Q ∨ free_in_prop x (x' ≡ value.num n), from free_in_prop.and.inv x_free_in_P,
+        or.elim this.symm
+        (
+          assume x_free_in_num: free_in_prop x (x' ≡ value.num n),
+          show ∃v, σ' x = some v, by begin
+            cases x_free_in_num,
+            case free_in_prop.term x_free_in_eq {
+              cases x_free_in_eq,
+              case free_in_term.binop₁ free_in_x' {
+                have x'_is_x: (x' = x), from (free_in_term.freevar.inv free_in_x').symm,
+                contradiction
+              },
+              case free_in_term.binop₂ free_in_num {
+                cases free_in_num
+              }
+            }
+          end
+        )
+        (
+          assume x_free_in_Q: free_in_prop x Q,
+          show ∃v, σ' x = some v, from ih x_free_in_Q
+        )
+      )
+    },
+    case env.vcgen.func σ₁ σ₂ f g fx R S e Q₁ Q₂ Q₃ σ₁_verified σ₂_verified func_verified _ ih₁ ih₂ { from
+      val_of_free_in_nonempty_env σ₁_verified (
+        assume f_is_not_x: f ≠ x,
+        have free_in_prop x (Q₁ & spec.func f fx R S) ∨ free_in_prop x (f ≡ value.func g fx R S e σ₂),
+        from free_in_prop.and.inv x_free_in_P,
+        or.elim this
+        (
+          assume x_free_in_Q₁_or_spec: free_in_prop x (Q₁ & spec.func f fx R S),
+          have free_in_prop x Q₁ ∨ free_in_prop x (spec.func f fx R S),
+          from free_in_prop.and.inv x_free_in_Q₁_or_spec,
+          or.elim this
+          (
+            assume x_free_in_Q₁: free_in_prop x Q₁,
+            show ∃v, σ₁ x = some v, from ih₁ x_free_in_Q₁
+          )
+          (
+            assume x_free_in_spec: free_in_prop x (spec.func f fx R S),
+            show ∃v, σ₁ x = some v, by begin
+              admit
+            end
+          )
+        )
+        (
+          assume x_free_in_func: free_in_prop x (f ≡ value.func g fx R S e σ₂),
+          show ∃v, σ₁ x = some v, by begin
+            cases x_free_in_func,
+            case free_in_prop.term x_free_in_eq {
+              cases x_free_in_eq,
+              case free_in_term.binop₁ free_in_f {
+                have f_is_x: (f = x), from (free_in_term.freevar.inv free_in_f).symm,
+                contradiction
+              },
+              case free_in_term.binop₂ free_in_func {
+                cases free_in_func
+              }
+            }
+          end
+        )
+      )
+    }
+  end
+
+theorem progress(H: list call) (s: stack): (H ⊩ s) → is_return s ∨ ∃c s', s ⟶ c, s'
 :=
-  assume ⟨P_valid, s_verified⟩,
+  assume s_verified: H ⊩ s,
   stack.vcgen.rec_on s_verified
   ( -- top
     assume (P₁ P₂: prop) (σ: env) (e: exp) (Q: propctx),
