props.lean
@@ -36,6 +36,141 @@ structure freevars := (p: prop)
 instance : has_mem var freevars := ⟨λx fv, free_in_prop x fv.p⟩ 
 def FV(p: prop): freevars := freevars.mk p
 
+-- helper lemmas
+
+lemma free_in_term.freevar.inv {x y: var}: free_in_term x y → (x = y) :=
+  assume x_free_in_y: free_in_term x y,
+  begin
+    cases x_free_in_y,
+    case free_in_term.freevar a b c { exact rfl }
+  end
+
+lemma free_in_prop.and.inv {P₁ P₂: prop} {x: var}: free_in_prop x (P₁ & P₂) → free_in_prop x P₁ ∨ free_in_prop x P₂ :=
+  assume x_free_in_and: free_in_prop x (P₁ & P₂),
+  begin
+    cases x_free_in_and,
+    case free_in_prop.and₁ free_in_P₁ {
+      show free_in_prop x P₁ ∨ free_in_prop x P₂, from or.inl free_in_P₁
+    },
+    case free_in_prop.and₂ free_in_P₂ {
+      show free_in_prop x P₁ ∨ free_in_prop x P₂, from or.inr free_in_P₂
+    }
+  end
+
+lemma call_history_closed (H: list call) (x: var): ¬ free_in_prop x (calls_to_prop H) :=
+  list.rec_on H
+  ( -- empty history
+    assume x_free: free_in_prop x (calls_to_prop list.nil),
+    have calls_to_prop list.nil = value.true, from rfl,
+    have x_free_in_true: free_in_prop x value.true, from this ▸ x_free,
+    show «false», by begin
+      cases x_free_in_true,
+      case free_in_prop.term x_free_in_term {
+        cases x_free_in_term
+      }
+    end
+  )
+  ( -- <call> :: rest
+    assume ⟨f, x', R, S, e, σ, vₓ, v⟩,
+    assume rest: list call,
+    assume ih: ¬ free_in_prop x (calls_to_prop rest),
+    assume x_free: free_in_prop x (calls_to_prop (⟨f, x', R, S, e, σ, vₓ, v⟩ :: rest)),
+    have calls_to_prop (⟨f, x', R, S, e, σ, vₓ, v⟩ :: rest) =
+      (prop.call (value.func f x' R S e σ) vₓ &
+      prop.post (value.func f x' R S e σ) vₓ &
+      term.app (value.func f x' R S e σ) vₓ ≡ v &
+      calls_to_prop rest), from rfl,
+    have x_free_in_prop: free_in_prop x (
+      prop.call (value.func f x' R S e σ) vₓ &
+      prop.post (value.func f x' R S e σ) vₓ &
+      term.app (value.func f x' R S e σ) vₓ ≡ v &
+      calls_to_prop rest), from this ▸ x_free,
+    have x_not_free_in_v: ¬ free_in_term x v, from (
+      assume x_free_in_v: free_in_term x v,
+      show «false», by cases x_free_in_v
+    ),
+    have x_not_free_in_vₓ: ¬ free_in_term x vₓ, from (
+      assume x_free_in_vₓ: free_in_term x vₓ,
+      show «false», by cases x_free_in_vₓ
+    ),
+    have x_not_free_in_f: ¬ free_in_term x (value.func f x' R S e σ), from (
+      assume x_free_in_f: free_in_term x (value.func f x' R S e σ),
+      show «false», by cases x_free_in_f
+    ),
+    have
+      free_in_prop x (calls_to_prop rest) ∨
+      free_in_prop x (prop.call (value.func f x' R S e σ) vₓ &
+        prop.post (value.func f x' R S e σ) vₓ &
+        term.app (value.func f x' R S e σ) vₓ ≡ v),
+    from (free_in_prop.and.inv x_free_in_prop).symm,
+    or.elim this ih (
+      assume x_free_in_call: free_in_prop x (
+        prop.call (value.func f x' R S e σ) vₓ &
+        prop.post (value.func f x' R S e σ) vₓ &
+        term.app (value.func f x' R S e σ) vₓ ≡ v),
+      have
+        free_in_prop x (term.app (value.func f x' R S e σ) vₓ ≡ v) ∨
+        free_in_prop x (prop.call (value.func f x' R S e σ) vₓ &
+          prop.post (value.func f x' R S e σ) vₓ),
+      from (free_in_prop.and.inv x_free_in_call).symm,
+      or.elim this (
+        assume x_free_in_eq_app: free_in_prop x (term.app (value.func f x' R S e σ) vₓ ≡ v),
+        show «false», by begin
+          cases x_free_in_eq_app,
+          case free_in_prop.term x_free_in_term {
+            cases x_free_in_term,
+            case free_in_term.binop₁ x_free_in_app {
+              cases x_free_in_app,
+              case free_in_term.app₁ x_free_in_f {
+                show «false», from x_not_free_in_f x_free_in_f
+              },
+              case free_in_term.app₂ x_free_in_vₓ {
+                show «false», from x_not_free_in_vₓ x_free_in_vₓ
+              }
+            },
+            case free_in_term.binop₂ x_free_in_v {
+              show «false», from x_not_free_in_v x_free_in_v
+            }
+          }
+        end
+      )
+      (
+        assume x_free_in_call_or_func: free_in_prop x (
+          prop.call (value.func f x' R S e σ) vₓ &
+          prop.post (value.func f x' R S e σ) vₓ),
+        have
+          free_in_prop x (prop.call (value.func f x' R S e σ) vₓ) ∨
+          free_in_prop x (prop.post (value.func f x' R S e σ) vₓ),
+        from free_in_prop.and.inv x_free_in_call_or_func,
+        or.elim this
+        (
+          assume x_free_in_call: free_in_prop x (prop.call (value.func f x' R S e σ) vₓ),
+          show «false», by begin
+            cases x_free_in_call,
+            case free_in_prop.call₁ x_free_in_f {
+              show «false», from x_not_free_in_f x_free_in_f
+            },
+            case free_in_prop.call₂ x_free_in_vₓ {
+              show «false», from x_not_free_in_vₓ x_free_in_vₓ
+            }
+          end
+        )
+        (
+          assume x_free_in_post: free_in_prop x (prop.post (value.func f x' R S e σ) vₓ),
+          show «false», by begin
+            cases x_free_in_post,
+            case free_in_prop.post₁ x_free_in_f {
+              show «false», from x_not_free_in_f x_free_in_f
+            },
+            case free_in_prop.post₂ x_free_in_vₓ {
+              show «false», from x_not_free_in_vₓ x_free_in_vₓ
+            }
+          end
+        )
+      )
+    )
+  )
+
 -- validity
 
 inductive valid : prop → Prop
